UPPAAL_State_Networks_Impl_Refine.thy
@@ -382,8 +382,9 @@ lemma steps_steps_approx':
   apply (case_tac x2)
    apply (simp split: option.split_asm if_split_asm)
    apply (case_tac x1)
-                   apply (auto split: if_split_asm; fail)
-                  apply (auto split: if_split_asm elim: UPPAAL_Asm.step.elims; fail)
+                    apply (auto split: if_split_asm; fail)
+                   apply (auto split: if_split_asm elim: UPPAAL_Asm.step.elims; fail)
+                  apply (auto elim!: UPPAAL_Asm.step.elims split: if_split_asm; fail)
                  apply (auto elim!: UPPAAL_Asm.step.elims split: if_split_asm; fail)
                 apply (auto elim!: UPPAAL_Asm.step.elims split: if_split_asm; fail)
                apply (auto elim!: UPPAAL_Asm.step.elims split: if_split_asm; fail)
@@ -428,9 +429,9 @@ lemma stepsc_steps_approx:
   shows "pc' \<in> steps_approx n prog pc"
   using assms
   apply (
-    induction "conv_prog P" n u "(pc, st, s, f, rs)" "(pc', st', s', f', rs')"
-    arbitrary: pc st s f rs rule: stepsc.induct
-    )
+      induction "conv_prog P" n u "(pc, st, s, f, rs)" "(pc', st', s', f', rs')"
+      arbitrary: pc st s f rs rule: stepsc.induct
+      )
    apply (simp split: option.split)
   apply clarsimp
   apply rule
@@ -441,8 +442,10 @@ lemma stepsc_steps_approx:
   apply (case_tac z)
    apply (simp split: option.split_asm if_split_asm)
    apply (case_tac x1)
-                  apply (simp split: if_split_asm)
-                 apply (auto elim: UPPAAL_Asm.step.elims)[]
+                    apply (simp split: if_split_asm)
+                   apply (auto elim: UPPAAL_Asm.step.elims)[]
+                  apply (auto elim!: UPPAAL_Asm.step.elims split: if_split_asm)[]
+                 apply (auto elim!: UPPAAL_Asm.step.elims split: if_split_asm)[]
                 apply (auto elim!: UPPAAL_Asm.step.elims split: if_split_asm)[]
                apply (auto elim!: UPPAAL_Asm.step.elims split: if_split_asm)[]
               apply (auto elim!: UPPAAL_Asm.step.elims split: if_split_asm)[]
@@ -453,7 +456,6 @@ lemma stepsc_steps_approx:
          apply (auto elim!: UPPAAL_Asm.step.elims split: if_split_asm)[]
         apply (auto elim!: UPPAAL_Asm.step.elims split: if_split_asm)[]
        apply (auto elim!: UPPAAL_Asm.step.elims split: if_split_asm)[]
-      apply (auto elim!: UPPAAL_Asm.step.elims split: if_split_asm)[]
        apply (case_tac "q < length prog")
         apply force
        apply (drule stepsc_out_of_range; simp)
@@ -862,7 +864,7 @@ lemma guaranteed_execution:
     "\<forall> pc \<in> {pc..<pc_t}.
       prog ! pc \<noteq> None
       \<and> prog ! pc \<notin> Some ` INSTR `
-        {HALT, POP, CALL, RETURN, instr.AND, instr.NOT, instr.ADD, instr.LT, instr.LE, instr.EQ}
+        {STORE, HALT, POP, CALL, RETURN, instr.AND, instr.NOT, instr.ADD, instr.LT, instr.LE, instr.EQ}
       \<and> (\<forall> c d. prog ! pc = Some (INSTR (STOREC c d)) \<longrightarrow> d = 0)
       "
     "\<forall> pc \<in> {pc..<pc_t}. \<forall> pc'. prog ! pc = Some (INSTR (JMPZ pc')) \<longrightarrow> pc' > pc \<and> pc' \<le> pc_t"
@@ -884,7 +886,7 @@ proof (induction "pc_t - pc" arbitrary: pc st s f r n rule: less_induct)
     case False
     with less.prems(1,4) have valid_instr:
       "prog ! pc \<notin> Some ` INSTR `
-            {HALT, POP, CALL, RETURN, instr.AND, instr.NOT, instr.ADD, instr.LT, instr.LE, instr.EQ}"
+       {STORE, HALT, POP, CALL, RETURN, instr.AND, instr.NOT, instr.ADD, instr.LT, instr.LE, instr.EQ}"
       "prog ! pc \<noteq> None"
       by auto
     from \<open>pc \<le> _\<close> \<open>pc_t \<noteq> _\<close> less.prems(2) have jumps:
@@ -975,13 +977,13 @@ lemma find_next_halt_finds_halt:
   if "find_next_halt prog pc = Some pc'"
 using that proof (induction prog pc rule: find_next_halt.induct)
   case prems: (1 prog pc)
-  from prems(19) show ?case
+  from prems(20) show ?case
     by (
         simp,
         simp
         split: if_split_asm option.split_asm instrc.split_asm instr.split_asm
         del: find_next_halt.simps;
-        fastforce dest: prems(1-18) simp del: find_next_halt.simps)
+        fastforce dest: prems(1-19) simp del: find_next_halt.simps)
 qed
 
 definition
@@ -993,7 +995,7 @@ definition
        \<forall> pc \<in> {pc_s..<pc_t}.
           prog ! pc \<noteq> None
           \<and> prog ! pc \<notin> Some ` INSTR `
-            {HALT, POP, CALL, RETURN, instr.AND, instr.NOT, instr.ADD, instr.LT, instr.LE, instr.EQ}
+            {STORE, HALT, POP, CALL, RETURN, instr.AND, instr.NOT, instr.ADD, instr.LT, instr.LE, instr.EQ}
           \<and> (\<forall> c d. prog ! pc = Some (INSTR (STOREC c d)) \<longrightarrow> d = 0)
         ) \<and>
         (\<forall> pc \<in> {pc_s..<pc_t}. \<forall> pc'. prog ! pc = Some (INSTR (JMPZ pc')) \<longrightarrow> pc' > pc \<and> pc' \<le> pc_t)
@@ -1009,7 +1011,7 @@ lemma guaranteed_execution_cond_alt_def[code]:
        \<forall> pc \<in> {pc_s..<pc_t}.
           prog ! pc \<noteq> None
           \<and> prog ! pc \<notin> Some ` INSTR `
-            {HALT, POP, CALL, RETURN, instr.AND, instr.NOT, instr.ADD, instr.LT, instr.LE, instr.EQ}
+            {STORE, HALT, POP, CALL, RETURN, instr.AND, instr.NOT, instr.ADD, instr.LT, instr.LE, instr.EQ}
           \<and> (case prog ! pc of Some (INSTR (STOREC c d)) \<Rightarrow> d = 0 | _ \<Rightarrow> True)
         ) \<and>
         (\<forall> pc \<in> {pc_s..<pc_t}.
